pcuic/theories/PCUICWeakeningEnv.v
@@ -51,8 +51,9 @@ Lemma leq_term_subset {cf:checker_flags} ctrs ctrs' t u
   : ConstraintSet.Subset ctrs ctrs' -> leq_term ctrs t u -> leq_term ctrs' t u.
 Proof.
   intro H. apply eq_term_upto_impl.
-  intros t' u'; eapply eq_universe_subset; assumption.
-  intros t' u'; eapply leq_universe_subset; assumption.
+  - intros t' u'. eapply eq_universe_subset. assumption.
+  - intros t' u'. eapply leq_universe_subset. assumption.
+  - intro. auto.
 Qed.
 
 (** * Weakening lemmas w.r.t. the global environment *)
@@ -101,6 +102,7 @@ Lemma eq_term_subset {cf:checker_flags} φ φ' t t'
     -> eq_term φ t t' ->  eq_term φ' t t'.
 Proof.
   intro H. apply eq_term_upto_impl.
+  3:{ intro. auto. }
   all: intros u u'; eapply eq_universe_subset; assumption.
 Qed.
 
